\documentclass{article}
\usepackage{lscape}
\usepackage{Sweave}
\begin{document}
\LARGE
\input{TablaHermite-concordance}
\thispagestyle{empty}
\begin{landscape}
\begin{center}
\begin{tabular}{llll}
\multicolumn{1}{c}{$z$} & \multicolumn{1}{c}{$f(z)$}&\multicolumn{1}{p{5cm}}{Primeras diferencias divididas}&\multicolumn{1}{p{5cm}}{Segundas diferencias divididas}\\\hline
$z_0=x_0$&$f[z_0]=f(x_0)$&&\\
&&$f[z_0,z_1]=f'(x_0)$&\\
$z_1=x_0$&$f[z_1]=f(x_0)$&&$f[z_0,z_1,z_2]=\frac{f[z_1,z_2]-f[z_0,z_1]}{z_2-z_0}$\\
&&$f[z_1,z_2]=\frac{f[z_2]-f[z_1]}{z_2-z_1}$&\\
$z_2=x_1$&$f[z_2]=f(x_1)$&&$f[z_1,z_2,z_3]=\frac{f[z_2,z_3]-f[z_1,z_2]}{z_3-z_1}$\\
&&$f[z_2,z_3]=f'(x_1)$&\\
$z_3=x_1$&$f[z_3]=f(x_1)$&&$f[z_2,z_3,z_4]=\frac{f[z_3,z_4]-f[z_2,z_3]}{z_4-z_2}$\\
&&$f[z_3,z_4]=\frac{f[z_4]-f[z_3]}{z_4-z_3}$&\\
$z_4=x_2$&$f[z_4]=f(x_2)$&&$f[z_3,z_4,z_5]=\frac{f[z_4,z_5]-f[z_3,z_4]}{z_5-z_3}$\\
&&$f[z_4,z_5]=f'(x_2)$&\\
$z_5=x_2$&$f[z_5]=f(x_2)$&&\\\hline
\end{tabular}
\end{center}
\end{landscape}


\end{document}
